code/ecdsap256/Hacl.Impl.P256.PointDouble.fsti
@@ -7,33 +7,20 @@ module ST = FStar.HyperStack.ST
 open Lib.IntTypes
 open Lib.Buffer
 
-open Hacl.Spec.P256.MontgomeryMultiplication
 open Hacl.Spec.P256.Bignum
 open Hacl.Impl.P256.Point
 
 module S = Spec.P256
+module SM = Hacl.Spec.P256.MontgomeryMultiplication
 
 #set-options "--z3rlimit 30 --fuel 0 --ifuel 0"
 
-val point_double: p:point -> result:point -> tempBuffer:lbuffer uint64 (size 88) -> Stack unit
-  (requires fun h -> live h p /\ live h tempBuffer /\ live h result /\
-    disjoint p tempBuffer /\ disjoint result tempBuffer /\
-    eq_or_disjoint p result /\
-    as_nat h (gsub p (size 8) (size 4)) < S.prime /\
-    as_nat h (gsub p (size 0) (size 4)) < S.prime /\
-    as_nat h (gsub p (size 4) (size 4)) < S.prime)
-  (ensures fun h0 _ h1 -> modifies (loc tempBuffer |+| loc result)  h0 h1 /\
-    as_nat h1 (gsub result (size 8) (size 4)) < S.prime /\
-    as_nat h1 (gsub result (size 0) (size 4)) < S.prime /\
-    as_nat h1 (gsub result (size 4) (size 4)) < S.prime /\
-    (
-      let x, y, z = gsub p (size 0) (size 4),  gsub p (size 4) (size 4), gsub p (size 8) (size 4) in
-      let x3, y3, z3 = gsub result (size 0) (size 4), gsub result (size 4) (size 4), gsub result (size 8) (size 4) in
-
-      let xD, yD, zD = fromDomain_ (as_nat h0 x), fromDomain_ (as_nat h0 y), fromDomain_ (as_nat h0 z) in
-      let x3D, y3D, z3D = fromDomain_ (as_nat h1 x3), fromDomain_ (as_nat h1 y3), fromDomain_ (as_nat h1 z3) in
-
-      let xN, yN, zN = S.point_double (xD, yD, zD) in
-      x3D == xN /\ y3D == yN /\ z3D == zN
-  )
-)
+val point_double: p:point -> res:point -> tmp:lbuffer uint64 (size 88) -> Stack unit
+  (requires fun h ->
+    live h p /\ live h tmp /\ live h res /\
+    disjoint p tmp /\ disjoint res tmp /\ eq_or_disjoint p res /\
+    point_inv h p)
+  (ensures fun h0 _ h1 -> modifies (loc tmp |+| loc res)  h0 h1 /\
+    point_inv h1 res /\
+    SM.fromDomainPoint (as_point_nat h1 res) ==
+      S.point_double (SM.fromDomainPoint (as_point_nat h0 p)))
