code/ecdsap256/Hacl.Impl.P256.PointMul.fsti
@@ -56,3 +56,15 @@ val point_mul_g_bytes: res:point -> scalar:lbuffer uint8 32ul -> Stack unit
     point_inv h1 res /\
     as_point_nat h1 res == S.norm_jacob_point
       (S.point_mul_g (BSeq.nat_from_bytes_be (as_seq h0 scalar))))
+
+
+val point_mul_double_g: res:point -> scalar1:felem -> scalar2:felem -> p:point -> Stack unit
+  (requires fun h ->
+    live h res /\ live h scalar1 /\ live h scalar2 /\ live h p /\
+    disjoint res scalar1 /\ disjoint res scalar2 /\ disjoint res p /\
+    disjoint p scalar1 /\ disjoint p scalar2 /\
+    point_inv h p /\ as_nat h scalar1 < pow2 256 /\ as_nat h scalar2 < pow2 256)
+  (ensures  fun h0 _ h1 -> modifies (loc res) h0 h1 /\
+    point_inv h1 res /\
+    SM.fromDomainPoint (as_point_nat h1 res) ==
+      S.point_mul_double_g (as_nat h0 scalar1) (as_nat h0 scalar2) (as_point_nat h0 p))
